

Proof Engineering for Program Logics in Isabelle/HOL

Lecture 2: Program Logics

Chelsea Edmonds

University of Western Australia

`chelsea.edmonds@uwa.edu.au`

ANU Logic Summer School 2025

Lectures:

- Basic reasoning on programs in Isabelle/HOL
- **Program Logics: Hoare and Rely-Guarantee**
- A side quest: intro to coinduction in Isabelle/HOL
- Formally defining Rely-guarantee reasoning
- Modular proofs in Isabelle/HOL

Mix of theory and Isabelle/HOL implementations/proofs.

Lecture 2 Overview

- What is a Program Logic?
- Hoare Logic: Intuition, Semantics, and Rules
- Hoare Logic: Soundness
- Hoare Logic in Isabelle
- Rely-Guarantee Logic

Acknowledgment: Hoare Logic Isabelle content inspired by Nipkow & Klein's Concrete Semantics textbook.

Program Logics: An Overview

What is a Program Logic?

A *program logic* is a formal language (based on mathematical logic) for expressing and proving various properties of programs.

Well-known examples

There are numerous existing program logics (and various extensions) that can target a variety of different program properties and environments. Some examples include:

- 1967 - 1969: Hoare Logic (or Floyd-Hoare Logic). [2]
- 1983: Rely-Guarantee Logic [3]
- 2000: Separation Logic [5]
- 2020: Incorrectness Logic [4]

Hoare Logic

Hoare Logic Intuition

For a sequential program, we can consider a *Hoare Triple*

$$\{P\} C \{Q\}$$

Where:

- P is a predicate that represents the *pre-condition*
- Q is a predicate that represents the *post-condition*
- C is the program.

The Hoare triple states that if the pre-condition P is satisfied on the initial program state, then *if* the program terminates, the post-condition Q will be satisfied.

Some Example Programs

Lets consider some basic example programs:

Listing 1: basic assignment

```
{ x = n }  
x := x + 1  
{ x = n + 1 }
```

Listing 2: basic swap

```
{ x = a  $\wedge$  y = b }  
t := x;  
x := y;  
y := t  
{ x = b  $\wedge$  y = a }
```

Partial vs Total Correctness

Our Hoare triple definition is dependent on *termination*. Hence it represents *partial correctness*.

Total correctness ($[P] C [Q]$) has the following two conditions:

- If a program C starts in a state satisfying P , then the program terminates
- When the program terminates, the state satisfies Q .

In other words:

$$\text{Total Correctness} = \text{Termination} + \text{Partial Correctness}$$

More examples...

Listing 3: Terminating Loop

```
{ n >= 0 }  
while n > 0 do  
  n := n - 1  
{ n = 0 }
```

Partial Correctness: ✓

Total Correctness: ✓

Listing 4: Divergent Loop

```
{ x >= 0 }  
while x >= 0 do  
  x := x + 1  
{ x < 0 }
```

Partial Correctness: ✓

Total Correctness: ✗

We'll focus on partial correctness for now.

A More Formal Semantics

More formally, for partial correctness, our Hoare triple is valid (\models) according to the following definition:

$$\models \{P\}C\{Q\} \longleftrightarrow (\forall s\ t. P\ s \wedge (c, s) \rightarrow^* (c', t) \wedge \text{final}(c', t) \longrightarrow Q\ t)$$

Syntactic vs Semantic Assertions

In our examples so far we've been using *syntactic* assertions, i.e.

$$\{x = n\}$$

is an assertion on a syntactic expression, such as `bexp`, which is nice and intuitive for simple examples.

However, in our formal semantics, it's it becomes much easier to reason using *semantic* assertions, i.e. predicates over a program state s . For example, the syntactic assertion above corresponds to the semantic assertion:

$$\{\lambda s. s(x) = n\}$$

A Hoare Logic Proof System

We can use inference rules to specify a formal proof system for Hoare logic.

Under this proof system, we use:

$$\vdash \{P\} C \{Q\}$$

means the Hoare triple $\{P\} C \{Q\}$ can be derived.

Some Useful Relation Notation

Some notes on notation, assuming P and Q are unary predicates.

- We use $<$ and $>$ to be the standard ordering on predicates. e.g. $P < Q$ means that $\forall s. P\ s \longrightarrow Q\ s$
- \sqcap and \sqcup denote the infimum and supremum in the lattice of predicates, which are component-wise conjunction and disjunction. e.g. $(P \sqcap Q)\ s = P\ s \wedge Q\ s$

Later we'll also be using binary predicates, e.g. R .

- $\text{refl } R$ means R is a reflexive relation, i.e. $\forall s. R\ s\ s$
- $\text{stable } P\ R$ means P is stable with respect to R , i.e. $\forall s\ s'. P\ s \wedge R\ s\ s' \longrightarrow P\ s'$

A Hoare Logic Proof System

$$\frac{}{\vdash \{P\} \text{ done } \{P\}} (\text{DoneH}) \qquad \frac{}{\vdash \{(\lambda s. P \ s[a/x])\} x ::= a \{P\}} (\text{AssignH})$$

$$\frac{\vdash \{P\} c_1 \{P'\} \qquad \vdash \{P'\} c_2 \{Q'\}}{\vdash \{P\} \text{ seq } c_1 \ c_2 \{Q\}} (\text{SeqH})$$

$$\frac{\vdash \{P \sqcap (\text{bval } t)\} c_1 \{Q\} \qquad \vdash \{P \sqcap (\neg (\text{bval } t))\} c_2 \{Q\}}{\vdash \{P\} \text{ if } t \ c_1 \ c_2 \{Q\}} (\text{IfH})$$

$$\frac{\vdash \{P \sqcap (\text{bval } t)\} c \{P\}}{\vdash \{P\} \text{ while } t \ c \{P \sqcap \neg \text{bval } t\}} (\text{WhileH})$$

Hoare Logic: Assignment Rule

Let's take a closer look at the Assignment Rule:

$$\frac{}{\vdash \{(\lambda s. P \ s[a/x])\} x ::= a \{P\}} \text{(AssignH)}$$

This can feel a little backwards, modifying the pre-condition instead of the post-condition. Why wouldn't the other way around work?

$$\frac{}{\vdash \{P\} x ::= a \{\lambda s. P \ s[a/x]\}} \text{(AssignHBad)}$$

Hoare Logic: Assignment Rule

Let's take a closer look at the Assignment Rule:

$$\frac{}{\vdash \{(\lambda s. P \ s[a/x])\} \ x ::= a \ \{P\}} \text{(AssignH)}$$

This can feel a little backwards, modifying the pre-condition instead of the post-condition. Why wouldn't the other way around work?

$$\frac{}{\vdash \{P\} \ x ::= a \ \{\lambda s. P \ s[a/x]\}} \text{(AssignHBad)}$$

We could use it to prove a triple like this is valid!

$$\{x = 0\} \ x ::= 1 \ \{1 = 0\}$$

The While Rule

$$\frac{\vdash \{P \sqcap (\text{bval } t)\} c \{P\}}{\vdash \{P\} \text{ while } t \text{ c } \{P \sqcap \neg \text{bval } t\}} (\text{WhileH})$$

In this rule P acts as a loop invariant.

- It is true at the beginning and end of every loop iteration
- If the loop terminates, the condition t must be false.

The Consequence Rule

$$\frac{\vdash \{P'\} c \{Q'\} \quad P \leq P' \quad Q' \leq Q}{\vdash \{P\} c \{Q\}} \text{ (MonoH)}$$

Figure 1: Consequence Rule

This allows us to

- Strengthen the pre-condition
- Weaken the post-condition.

Deriving Rules

We can derive rules, that might be easier to work with. For example, here is an alternate rule for Assign:

$$\frac{\forall s. P \ s \longrightarrow Q \ s[a/x]}{\vdash \{P\} \ x ::= a \ \{Q\}} \text{(AssignH')}$$

Figure 2: Derived Assign Rule

This is derived via the consequence rule (strengthen the precondition), and original AssignH rule.

And for while:

$$\frac{\vdash \{P \sqcap (\text{bval } t)\} \ c \ \{P\} \qquad P \sqcap (\neg (\text{bval } t)) \leq Q}{\vdash \{P\} \ \text{while } t \ c \ \{Q\}} \text{(WhileH')}$$

Figure 3: Derived While Rule

Isabelle Demo

Soundness and Completeness

There are two important properties we typically want to consider when developing a program logic proof system w.r.t. an operational semantics.

First is *Soundness*: if a triple is derivable, then it is also valid.

$$\vdash \{P\} c \{Q\} \longrightarrow \models \{P\} c \{Q\}$$

Next is *Completeness*: if a triple is valid, then it is also derivable.

$$\models \{P\} c \{Q\} \longrightarrow \vdash \{P\} c \{Q\}$$

We'll focus on soundness proofs in this course. Completeness requires the introduction of the weakest pre-condition, which is left as further reading.

Isabelle Demo

Rely-Guarantee Logic

Additional Concurrency Considerations

For reasoning on the correctness of concurrent programs, we also need to consider:

- What do we *require* of the environment for a given sequential command to hold.
- How could our sequential command *impact* the environment.

The Rely-Guarantee Approach

Rely-Guarantee Logic extends Hoare Logic to reason about concurrent programs:

$$\{P, R\} C \{G, Q\}$$

Where C , P and Q are as before, and:

- R a binary predicate representing the *rely-condition*.
- G is a binary predicate representing the *guarantee-condition*.

Our triple now also requires that the environment only makes changes to the state that satisfy the rely-condition R , and that the program only makes changes to the state that satisfy the guarantee-condition G .

We focus on *partial correctness* again.

The Rely-Guarantee Approach

Slightly more formally, consider a command whose execution trace has environment steps $\epsilon(\sigma_i, \sigma_{i+1})$ and program steps $\tau(\sigma_i, \sigma_{i+1})$, where σ_i represents the state after i steps:

$$\sigma_0 \dots \tau(\sigma_i, \sigma_{i+1}) \dots \epsilon(\sigma_j, \sigma_{j+1}) \dots \sigma_f$$

$\{P, R\} C \{G, Q\}$ holds means:

- $P \sigma_0$ holds
- $Q \sigma_f$ holds if the command terminates
- Every environment step ϵ satisfies the rely condition, i.e. $R \sigma_j \sigma_{j+1}$
- Every program step τ satisfies the guarantee condition, i.e. $G \sigma_i \sigma_{i+1}$

An (Intuitive) Assignment Example

Consider the below Hoare triple:

Listing 5: basic assignment RG

```
{ x = 0 }  
x := x + 1  
{ x = 1 }
```

Say this command is running in a parallel environment. For it to hold under our RG logic, we additionally:

- *rely* on the condition that x is not changed by the environment.
- *guarantee* that our program at most increments x by 1.

A rely-guarantee proof system

$$\frac{\text{stable } Q \ R \quad P \leq Q}{\vdash \{P, R\} \text{ done } \{G, Q\}} \text{ (DoneRG)}$$

$$\frac{\begin{array}{c} \text{stable } P \ R \\ (\lambda s'. \exists s. P \ s \wedge s' = s[a/x]) \leq Q \end{array} \quad \begin{array}{c} \text{stable } Q \ R \\ (\lambda s, s'. P \ s \wedge s' = s[a/x]) \leq G \end{array}}{\vdash \{P, R\} \ x := a \ \{G, Q\}} \text{ (AssignRG)}$$

$$\frac{\vdash \{P, R\} \ c_1 \ \{G, P'\} \quad \vdash \{P', R\} \ c_2 \ \{G, Q\} \quad \text{refl } G}{\vdash \{P, R\} \text{ seq } c_1 \ c_2 \ \{G, Q\}} \text{ (SeqRG)}$$

A rely guarantee proof system

$$\frac{\begin{array}{c} \vdash \{ P \sqcap (\text{bval } t), R \} c_1 \{ G, Q \} \quad \vdash \{ P \sqcap (\neg (\text{bval } t)), R \} c_2 \{ G, Q \} \\ \text{stable } P \ R \quad \text{refl } G \end{array}}{\vdash \{ P, R \} \text{if } t \ c_1 \ c_2 \{ G, Q \}} \text{ (IfRG)}$$

$$\frac{\begin{array}{c} \vdash \{ P \sqcap (\text{bval } t), R \} c \{ G, P \} \quad P \sqcap (\neg (\text{bval } t)) \leq Q \\ \text{stable } P \ R \quad \text{stable } Q \ R \quad \text{refl } G \end{array}}{\vdash \{ P, R \} \text{while } t \ c \{ G, Q \}} \text{ (WhileRG)}$$

$$\frac{\begin{array}{c} \vdash \{ P_1, R_1 \} c_1 \{ G_1, Q_1 \} \quad \vdash \{ P_2, R_2 \} c_2 \{ G_2, Q_2 \} \\ P \leq P_1 \sqcap P_2 \quad R \sqcup G_2 \leq R_1 \quad R \sqcup G_1 \leq R_2 \\ G_1 \sqcup G_2 \leq G \quad Q_1 \sqcap Q_2 \leq Q \quad \text{refl } G \end{array}}{\vdash \{ P, R \} \text{par } c_1 \ c_2 \{ G, Q \}} \text{ (ParRG)}$$

The Parallel Rule

$$\frac{\begin{array}{c} \vdash \{ P_1, R_1 \} c_1 \{ G_1, Q_1 \} \quad \vdash \{ P_2, R_2 \} c_2 \{ G_2, Q_2 \} \\ P \leq P_1 \sqcap P_2 \quad R \sqcup G_2 \leq R_1 \quad R \sqcup G_1 \leq R_2 \\ G_1 \sqcup G_2 \leq G \quad Q_1 \sqcap Q_2 \leq Q \quad \text{refl } G \end{array}}{\vdash \{ P, R \} \text{ par } c_1 c_2 \{ G, Q \}} \text{(ParRG)}$$

The parallel rule is our critical new rule in the rely-guarantee reasoning proof system. It states for a parallel step to be derived:

- Both c_1 and c_2 satisfy their respective RG tuples.
- The precondition is equivalent to (or stronger) than the conjunction of P_1 and P_2
- The postcondition is equivalent to (or weaker) than the conjunction of Q_1 and Q_2
- The guarantee condition is equivalent to (or weaker) than the disjunction of G_1 and G_2
- G_2 is compatible with R_1
- G_1 is compatible with R_2

An example: Rely-Guarantee Conditions

Consider $c1$ where:

- $G1\ s\ s' \equiv s\ y = s'\ y$
- $R1\ s\ s' \equiv s'\ x < s\ x$

and $c2$ where:

- $G2\ s\ s' \equiv s'\ x < s\ x$
- $R2\ s\ s' \equiv s'\ y \geq s\ y$

Clearly we have that:

$$G2\ s\ s' \longrightarrow R1\ s\ s' \wedge G1\ s\ s' \longrightarrow R2\ s\ s'$$

So $c1$ and $c2$ could run in parallel with no interference issues.

The Rely-Guarantee Consequence Rule

$$\frac{\vdash \{P', R'\} c \{G', Q'\} \quad P \leq P' \quad R \leq R' \quad G' \leq G \quad Q' \leq Q}{\vdash \{P, R\} c \{G, Q\}} \text{(MonoRG)}$$

Figure 4: Rely-Guarantee Consequence Rule

Isabelle Demo

Rely-Guarantee Semantics?

Ok, so we have a proof system - but what about our formal Rely-Guarantee semantics?
i.e. how do we define:

$$\models \{P, R\} c \{G, Q\}$$

Concurrency introduces some challenges for a formal definition:

- How do we model environment vs program steps?
- How do we capture the rely/guarantee conditions?

We hinted out this with our slightly more formal definition earlier.

Rely-Guarantee Semantics Approaches

Multiple approaches exist to address these challenges, including:

- Trace-Based
- Reachability
- Inductive
- Coinductive?

We'll discuss these in more detail in Lecture 4.

Note: other approaches to rely-guarantee reasoning also exist, including a more algebraic refinement calculus style of reasoning by Hayes et al [1], and extensions such as total correctness and relational post-conditions.

Next Lecture: A side quest into coinduction!

- What is coinduction?
- How does it relate to inductive principles?
- How do we work with coinduction in Isabelle?
- We'll return to Rely-Guarantee in Isabelle in Lecture 4.

Isabelle exercises/extended work

Hoare Logic is covered in Chapter 12 of the Concrete Semantics Textbook.

- Try out some of the exercises from section 12.1/12.2
- Read up on weakest pre-conditions and potential for automation (section 12.4)

-  Ian J. Hayes and Cliff B. Jones.
A guide to rely/guarantee thinking.
In Jonathan P. Bowen, Zhiming Liu, and Zili Zhang, editors, *Engineering Trustworthy Software Systems*, pages 1–38, Cham, 2018. Springer International Publishing.
-  C. A. R. Hoare.
An axiomatic basis for computer programming.
Commun. ACM, 12(10):576–580, October 1969.
-  Cliff B. Jones.
Specification and design of (parallel) programs.
In *IFIP Congress*, 1983.



Peter W. O'Hearn.

Incorrectness logic.

Proc. ACM Program. Lang., 4(POPL), December 2019.



John C. Reynolds.

Separation logic: A logic for shared mutable data structures.

In *Proceedings of the 17th Annual IEEE Symposium on Logic in Computer Science*, LICS '02, page 55–74, USA, 2002. IEEE Computer Society.